Prove wrappers for read/write using seq<Block>

src/Dafny/examples/fs/block_fs.dfy
@@ -9,6 +9,7 @@ module BlockFs
   import opened JrnlSpec
   import opened IndirectPos
   import opened IndFs
+  import Inode
   import C = Collections
 
   datatype preInodeData = InodeData(blks: seq<Block>)
@@ -32,46 +33,114 @@ module BlockFs
     InodeData(blks)
   }
 
-  class BlockFilesys
+  predicate is_lba(i: int)
   {
-    ghost var data: map<Ino, InodeData>
-    const ifs: IndFilesys;
+    0 <= i < config.total
+  }
 
+  function block_data(data: imap<Pos, Block>): map<Ino, InodeData>
+    requires data_dom(data)
+  {
+    map ino:Ino | ino_ok(ino) :: inode_data(ino, data)
+  }
 
-    function metadata(): map<Ino, uint64>
-      reads ifs
+  method New(d: Disk) returns (fs: IndFilesys)
+    ensures fs.ValidQ()
+    ensures block_data(fs.data) == map ino: Ino | ino_ok(ino) :: InodeData.zero
+  {
+    fs := new IndFilesys(d);
+    assert forall ino: Ino | ino_ok(ino) :: inode_data(ino, fs.data) == InodeData.zero;
+  }
+
+  // public
+  method Read(fs: IndFilesys, txn: Txn, ino: Ino, n: nat)
+    returns (bs: Bytes)
+    modifies fs.fs
+    requires fs.ValidQ() ensures fs.ValidQ()
+    requires fs.has_jrnl(txn)
+    requires ino_ok(ino)
+    requires is_lba(n)
+    ensures bs.data == block_data(fs.data)[ino].blks[n]
+    // this should be unnecessary due to the precise modifies clause
+    // ensures fs.state_unchanged()
+  {
+    var i := fs.startInode(txn, ino);
+    bs := fs.read(txn, Pos.from_flat(ino, n), i);
+    fs.finishInodeReadonly(ino, i);
+  }
+
+  lemma map_update_eq<K,V>(m1: map<K, V>, k0: K, v: V, m2: map<K, V>)
+    requires forall k: K :: k in m1 <==> k in m2
+    requires forall k: K | k in m1 && k != k0 :: m1[k] == m2[k]
+    requires k0 in m2 && m2[k0] == v
+    ensures m2 == m1[k0 := v]
+  {}
+
+  lemma block_data_update(data: imap<Pos, Block>, ino: Ino, n: nat, blk: Block)
+    requires ino_ok(ino)
+    requires is_lba(n)
+    requires data_dom(data)
+    ensures inode_data(ino, data[Pos.from_flat(ino, n) := blk]).blks ==
+            inode_data(ino, data).blks[n := blk]
+  {
+    ghost var data' := data[Pos.from_flat(ino, n) := blk];
+    ghost var n0 := n;
+    ghost var d0 := inode_data(ino, data);
+    ghost var d := inode_data(ino, data');
+    forall n | is_lba(n)
+      ensures d.blks[n] == d0.blks[n0 := blk][n]
     {
-      ifs.metadata
+      if n == n0 {}
+      else {
+        assert Idx.from_flat(n) != Idx.from_flat(n0) by {
+          Idx.from_flat_inj(n, n0);
+        }
+      }
+    }
+  }
+
+  // an update to an ino0 Pos doesn't affect ino
+  lemma block_data_update_other(data: imap<Pos, Block>, ino0: Ino, ino: Ino, n: nat, blk: Block)
+    requires ino_ok(ino0) && ino_ok(ino) && ino0 != ino
+    requires is_lba(n)
+    requires data_dom(data)
+    ensures inode_data(ino, data[Pos.from_flat(ino0, n) := blk]) ==
+            inode_data(ino, data)
+  {}
+
+  // public
+  method Write(fs: IndFilesys, txn: Txn, ino: Ino, i: Inode.Inode, n: nat, blk: Bytes)
+    returns (ok: bool, i': Inode.Inode)
+    modifies fs.Repr()
+    requires fs.ValidIno(ino, i) ensures fs.ValidIno(ino, i')
+    requires fs.has_jrnl(txn)
+    requires is_lba(n)
+    requires is_block(blk.data)
+    ensures fs.metadata == old(fs.metadata)
+    ensures ok ==> block_data(fs.data) == (
+        var data := old(block_data(fs.data));
+        var d0 := data[ino];
+        data[ino := d0.(blks := d0.blks[n := blk.data])])
+    ensures !ok ==> block_data(fs.data) == old(block_data(fs.data))
+  {
+    ok, i' := fs.write(txn, Pos.from_flat(ino, n), i, blk);
+    if !ok {
+      return;
     }
 
-    function Repr(): set<object>
-    {
-      {this} + ifs.Repr()
+    assert blk.data == old(blk.data);
+
+    ghost var d0 := old(block_data(fs.data)[ino]);
+    ghost var d := block_data(fs.data)[ino];
+    assert d.blks == d0.blks[n := blk.data] by {
+      block_data_update(old(fs.data), ino, n, blk.data);
     }
 
-    predicate {:opaque} ValidData()
-      reads Repr()
-      requires ifs.ValidQ()
+    ghost var ino0 := ino;
+    forall ino:Ino | ino_ok(ino) && ino != ino0
+      ensures block_data(fs.data)[ino] == old(block_data(fs.data)[ino])
     {
-      && Fs.ino_dom(data)
-      && forall ino: Ino | ino_ok(ino) :: data[ino] == inode_data(ino, ifs.data)
-    }
-
-    predicate Valid()
-      reads Repr()
-    {
-      && ifs.ValidQ()
-      && ValidData()
-    }
-
-    constructor(d: Disk)
-      ensures Valid()
-      ensures data == map ino: Ino | ino_ok(ino) :: InodeData.zero
-    {
-      this.ifs := new IndFilesys(d);
-      this.data := map ino: Ino | ino_ok(ino) :: InodeData.zero;
-      new;
-      reveal ValidData();
+      block_data_update_other(old(fs.data), ino0, ino, n, blk.data);
     }
   }
 }
